pulse/lib/pulse/core/PulseCore.HeapSig.fst
@@ -1,0 +1,28 @@
+module PulseCore.HeapSig
+open FStar.Ghost
+open FStar.PCM
+module H2 = PulseCore.Heap2
+module ST = PulseCore.HoareStateMonad
+module CM = FStar.Algebra.CommMonoid
+
+let exists_ #h #a p = h.as_slprop (fun m -> exists (x:a). h.interp (p x) m)
+let interp_exists (#h:heap_sig u#h) (#a:Type u#a) (p: a -> h.slprop)
+: Lemma (forall m. h.interp (exists_ p) m <==> (exists x. h.interp (p x) m))
+= h.interp_as (fun m -> exists (x:a). h.interp (p x) m)
+
+let erase_cm (#a:Type) (c:CM.cm a)
+: CM.cm (erased a)
+= CM.CM (hide c.unit)
+        (fun x y -> hide (c.mult (reveal x) (reveal y)))
+        (fun x -> c.identity (reveal x))
+        (fun x y z -> c.associativity (reveal x) (reveal y) (reveal z))
+        (fun x y -> c.commutativity (reveal x) (reveal y))
+
+let cm_slprop (hs:heap_sig u#h) 
+: c:CM.cm (hs.slprop) { c.unit == hs.emp /\ c.mult == hs.star }
+= CM.CM hs.emp
+        hs.star
+        (fun x -> hs.emp_unit x; hs.star_commutative x hs.emp)
+        hs.star_associative hs.star_commutative
+
+let cm_e_slprop (hs:heap_sig u#h) = erase_cm (cm_slprop hs)
